feat: some translation and some equality theorem

CurryHowardCorrespondence/Varset.lean
@@ -13,7 +13,7 @@ def propVarNames.eq: propVarNames → propVarNames → Bool
 | propVarNames.s, propVarNames.s => true
 | _, _ => false
 
-instance : BEq propVarNames := ⟨propVarNames.eq⟩
+instance provpvarbeq : BEq propVarNames := ⟨propVarNames.eq⟩
 
 def propVarNames.toString: propVarNames → String
 | propVarNames.p => "p"
@@ -34,7 +34,7 @@ def typeVarNames.eq: typeVarNames → typeVarNames → Bool
 | typeVarNames.z, typeVarNames.z => true
 | _, _ => false
 
-instance : BEq typeVarNames := ⟨typeVarNames.eq⟩
+instance typevarbeq: BEq typeVarNames := ⟨typeVarNames.eq⟩
 
 def typeVarNames.toString: typeVarNames → String
 | typeVarNames.w => "w"
@@ -55,10 +55,294 @@ def termVarNames.eq: termVarNames → termVarNames → Bool
 | termVarNames.Z, termVarNames.Z => true
 | _, _ => false
 
-instance : BEq termVarNames := ⟨termVarNames.eq⟩
+instance termvarbeq : BEq termVarNames := ⟨termVarNames.eq⟩
 
 def termVarNames.toString: termVarNames → String
 | termVarNames.W => "W"
 | termVarNames.X => "X"
 | termVarNames.Y => "Y"
 | termVarNames.Z => "Z"
+
+def typeVarNames.fromPropVarNames: propVarNames → typeVarNames
+| propVarNames.p => typeVarNames.w
+| propVarNames.q => typeVarNames.x
+| propVarNames.r => typeVarNames.y
+| propVarNames.s => typeVarNames.z
+
+theorem eq_pvname_eq_tvname_: ∀ {p q}, p.eq q → (typeVarNames.fromPropVarNames p).eq (typeVarNames.fromPropVarNames q):= by
+  intro p q h
+  cases p
+  cases q
+  simp [typeVarNames.fromPropVarNames]
+  simp [typeVarNames.eq]
+  simp [propVarNames.eq] at h
+  simp [propVarNames.eq] at h
+  simp [propVarNames.eq] at h
+  cases q
+  simp [propVarNames.eq] at h
+  simp [typeVarNames.fromPropVarNames]
+  simp [typeVarNames.eq]
+  simp [propVarNames.eq] at h
+  simp [propVarNames.eq] at h
+  cases q
+  simp [propVarNames.eq] at h
+  simp [propVarNames.eq] at h
+  simp [typeVarNames.fromPropVarNames]
+  simp [typeVarNames.eq]
+  simp [propVarNames.eq] at h
+  cases q
+  simp [propVarNames.eq] at h
+  simp [propVarNames.eq] at h
+  simp [propVarNames.eq] at h
+  simp [typeVarNames.fromPropVarNames]
+  simp [typeVarNames.eq]
+
+theorem eq_tvname_eq_pvname_: ∀ {p q}, (typeVarNames.fromPropVarNames p).eq (typeVarNames.fromPropVarNames q) → p.eq q := by
+  intro p q h
+  cases p
+  cases q
+  simp [propVarNames.eq]
+  simp [typeVarNames.fromPropVarNames] at h
+  simp [typeVarNames.eq] at h
+  simp [typeVarNames.fromPropVarNames] at h
+  simp [typeVarNames.eq] at h
+  simp [typeVarNames.fromPropVarNames] at h
+  simp [typeVarNames.eq] at h
+  cases q
+  simp [typeVarNames.fromPropVarNames] at h
+  simp [typeVarNames.eq] at h
+  simp [propVarNames.eq]
+  simp [typeVarNames.fromPropVarNames] at h
+  simp [typeVarNames.eq] at h
+  simp [typeVarNames.fromPropVarNames] at h
+  simp [typeVarNames.eq] at h
+  cases q
+  simp [typeVarNames.fromPropVarNames] at h
+  simp [typeVarNames.eq] at h
+  simp [typeVarNames.fromPropVarNames] at h
+  simp [typeVarNames.eq] at h
+  simp [propVarNames.eq]
+  simp [typeVarNames.fromPropVarNames] at h
+  simp [typeVarNames.eq] at h
+  cases q
+  simp [typeVarNames.fromPropVarNames] at h
+  simp [typeVarNames.eq] at h
+  simp [typeVarNames.fromPropVarNames] at h
+  simp [typeVarNames.eq] at h
+  simp [typeVarNames.fromPropVarNames] at h
+  simp [typeVarNames.eq] at h
+  simp [propVarNames.eq]
+
+theorem eq_pvname_eq_tvname: ∀ {p q}, p == q → (typeVarNames.fromPropVarNames p) == (typeVarNames.fromPropVarNames q):= by
+  intro p q h
+  simp [provpvarbeq] at h
+  simp [typevarbeq]
+  rw [eq_pvname_eq_tvname_]
+  exact h
+
+theorem eq_tvname_eq_pvname: ∀ {p q}, (typeVarNames.fromPropVarNames p) == (typeVarNames.fromPropVarNames q) → p == q := by
+  intro p q h
+  simp [typevarbeq] at h
+  simp [provpvarbeq]
+  rw [eq_tvname_eq_pvname_]
+  exact h
+
+def typeVarNames.toPropVarNames: typeVarNames → propVarNames
+| typeVarNames.w =>  propVarNames.p
+| typeVarNames.x =>  propVarNames.q
+| typeVarNames.y =>  propVarNames.r
+| typeVarNames.z =>  propVarNames.s
+
+theorem eq_tvname_eq_pvname2: ∀ {p q:typeVarNames}, p==q → p.toPropVarNames == q.toPropVarNames := by
+  intro p q h
+  simp [typevarbeq] at h
+  simp [provpvarbeq]
+  cases q
+  cases p
+  simp [typeVarNames.toPropVarNames]
+  simp [propVarNames.eq]
+  simp [typeVarNames.eq] at h
+  simp [typeVarNames.eq] at h
+  simp [typeVarNames.eq] at h
+  cases p
+  simp [typeVarNames.eq] at h
+  simp [typeVarNames.toPropVarNames]
+  simp [propVarNames.eq]
+  simp [typeVarNames.eq] at h
+  simp [typeVarNames.eq] at h
+  cases p
+  simp [typeVarNames.eq] at h
+  simp [typeVarNames.eq] at h
+  simp [typeVarNames.toPropVarNames]
+  simp [propVarNames.eq]
+  simp [typeVarNames.eq] at h
+  cases p
+  simp [typeVarNames.eq] at h
+  simp [typeVarNames.eq] at h
+  simp [typeVarNames.eq] at h
+  simp [typeVarNames.toPropVarNames]
+  simp [propVarNames.eq]
+
+theorem eq_pvname_eq_tvname2: ∀ {p q:typeVarNames}, p.toPropVarNames == q.toPropVarNames → p==q := by
+  intro p q h
+  simp [typevarbeq]
+  simp [provpvarbeq] at h
+  cases p
+  cases q
+  simp [typeVarNames.eq]
+  simp [typeVarNames.toPropVarNames,propVarNames.eq] at h
+  simp [typeVarNames.toPropVarNames,propVarNames.eq] at h
+  simp [typeVarNames.toPropVarNames,propVarNames.eq] at h
+  cases q
+  simp [typeVarNames.toPropVarNames,propVarNames.eq] at h
+  simp [typeVarNames.eq]
+  simp [typeVarNames.toPropVarNames,propVarNames.eq] at h
+  simp [typeVarNames.toPropVarNames,propVarNames.eq] at h
+  cases q
+  simp [typeVarNames.toPropVarNames,propVarNames.eq] at h
+  simp [typeVarNames.toPropVarNames,propVarNames.eq] at h
+  simp [typeVarNames.eq]
+  simp [typeVarNames.toPropVarNames,propVarNames.eq] at h
+  cases q
+  simp [typeVarNames.toPropVarNames,propVarNames.eq] at h
+  simp [typeVarNames.toPropVarNames,propVarNames.eq] at h
+  simp [typeVarNames.toPropVarNames,propVarNames.eq] at h
+  simp [typeVarNames.eq]
+
+
+def termVarNames.fromPropVarNames: propVarNames → termVarNames
+| propVarNames.p => termVarNames.W
+| propVarNames.q => termVarNames.X
+| propVarNames.r => termVarNames.Y
+| propVarNames.s => termVarNames.Z
+
+theorem eq_pvname_eq_tname: ∀ {p q}, p == q → (termVarNames.fromPropVarNames p) == (termVarNames.fromPropVarNames q):= by
+  intro p q h
+  simp [termvarbeq]
+  simp [provpvarbeq] at h
+  cases p
+  cases q
+  simp [termVarNames.fromPropVarNames]
+  simp [termVarNames.eq]
+  simp [propVarNames.eq] at h
+  simp [propVarNames.eq] at h
+  simp [propVarNames.eq] at h
+  cases q
+  simp [propVarNames.eq] at h
+  simp [termVarNames.fromPropVarNames]
+  simp [termVarNames.eq]
+  simp [propVarNames.eq] at h
+  simp [propVarNames.eq] at h
+  cases q
+  simp [propVarNames.eq] at h
+  simp [propVarNames.eq] at h
+  simp [termVarNames.fromPropVarNames]
+  simp [termVarNames.eq]
+  simp [propVarNames.eq] at h
+  cases q
+  simp [propVarNames.eq] at h
+  simp [propVarNames.eq] at h
+  simp [propVarNames.eq] at h
+  simp [termVarNames.fromPropVarNames]
+  simp [termVarNames.eq]
+
+theorem eq_tname_eq_pvname: ∀ {p q}, (termVarNames.fromPropVarNames p)== (termVarNames.fromPropVarNames q) → p ==q := by
+  intro p q h
+  simp [termvarbeq] at h
+  simp [provpvarbeq]
+  cases p
+  cases q
+  simp [propVarNames.eq]
+  simp [termVarNames.fromPropVarNames] at h
+  simp [termVarNames.eq] at h
+  simp [termVarNames.fromPropVarNames] at h
+  simp [termVarNames.eq] at h
+  simp [termVarNames.fromPropVarNames] at h
+  simp [termVarNames.eq] at h
+  cases q
+  simp [termVarNames.fromPropVarNames] at h
+  simp [termVarNames.eq] at h
+  simp [propVarNames.eq]
+  simp [termVarNames.fromPropVarNames] at h
+  simp [termVarNames.eq] at h
+  simp [termVarNames.fromPropVarNames] at h
+  simp [termVarNames.eq] at h
+  cases q
+  simp [termVarNames.fromPropVarNames] at h
+  simp [termVarNames.eq] at h
+  simp [termVarNames.fromPropVarNames] at h
+  simp [termVarNames.eq] at h
+  simp [propVarNames.eq]
+  simp [termVarNames.fromPropVarNames] at h
+  simp [termVarNames.eq] at h
+  cases q
+  simp [termVarNames.fromPropVarNames] at h
+  simp [termVarNames.eq] at h
+  simp [termVarNames.fromPropVarNames] at h
+  simp [termVarNames.eq] at h
+  simp [termVarNames.fromPropVarNames] at h
+  simp [termVarNames.eq] at h
+  simp [propVarNames.eq]
+
+
+def termVarNames.toPropVarNames: termVarNames → propVarNames
+| termVarNames.W =>  propVarNames.p
+| termVarNames.X =>  propVarNames.q
+| termVarNames.Y =>  propVarNames.r
+| termVarNames.Z =>  propVarNames.s
+
+theorem eq_tname_eq_pvname2: ∀ {p q:termVarNames}, p==q → p.toPropVarNames == q.toPropVarNames := by
+  intro p q h
+  simp [termvarbeq] at h
+  simp [provpvarbeq]
+  cases q
+  cases p
+  simp [termVarNames.toPropVarNames]
+  simp [propVarNames.eq]
+  simp [termVarNames.eq] at h
+  simp [termVarNames.eq] at h
+  simp [termVarNames.eq] at h
+  cases p
+  simp [termVarNames.eq] at h
+  simp [termVarNames.toPropVarNames]
+  simp [propVarNames.eq]
+  simp [termVarNames.eq] at h
+  simp [termVarNames.eq] at h
+  cases p
+  simp [termVarNames.eq] at h
+  simp [termVarNames.eq] at h
+  simp [termVarNames.toPropVarNames]
+  simp [propVarNames.eq]
+  simp [termVarNames.eq] at h
+  cases p
+  simp [termVarNames.eq] at h
+  simp [termVarNames.eq] at h
+  simp [termVarNames.eq] at h
+  simp [termVarNames.toPropVarNames]
+  simp [propVarNames.eq]
+
+theorem eq_pvname_eq_tname2: ∀ {p q:termVarNames}, p.toPropVarNames == q.toPropVarNames → p==q := by
+  intro p q h
+  simp [termvarbeq]
+  simp [provpvarbeq] at h
+  cases p
+  cases q
+  simp [termVarNames.eq]
+  simp [termVarNames.toPropVarNames,propVarNames.eq] at h
+  simp [termVarNames.toPropVarNames,propVarNames.eq] at h
+  simp [termVarNames.toPropVarNames,propVarNames.eq] at h
+  cases q
+  simp [termVarNames.toPropVarNames,propVarNames.eq] at h
+  simp [termVarNames.eq]
+  simp [termVarNames.toPropVarNames,propVarNames.eq] at h
+  simp [termVarNames.toPropVarNames,propVarNames.eq] at h
+  cases q
+  simp [termVarNames.toPropVarNames,propVarNames.eq] at h
+  simp [termVarNames.toPropVarNames,propVarNames.eq] at h
+  simp [termVarNames.eq]
+  simp [termVarNames.toPropVarNames,propVarNames.eq] at h
+  cases q
+  simp [termVarNames.toPropVarNames,propVarNames.eq] at h
+  simp [termVarNames.toPropVarNames,propVarNames.eq] at h
+  simp [termVarNames.toPropVarNames,propVarNames.eq] at h
+  simp [termVarNames.eq]
